\section*{Problem 1}
\begin{align*}
	\mathbf{A} = 
	\begin{pmatrix}
	-1 & 1 \\
	1 & -1
	\end{pmatrix}
	,\quad
	\mathbf{B} = \frac{1}{\sqrt{5}}
	\begin{pmatrix}
	-1 & 2 \\
	2 & 1
	\end{pmatrix}
\end{align*}

\subsection*{a) Eigenvalues}
\begin{align*}
	\det\left(\lambda\mathbf{I-A}\right)\overset{!}{=}0
	\quad&\rightarrow
	\begin{vmatrix}
	\lambda+1 & 1 \\
	1 & \lambda +1
	\end{vmatrix}
	\overset{!}{=}0& \\
	&\Rightarrow\lambda_{1}^{A}=-2,\quad\lambda_{2}^{A}=0& \\
	\det\left(\lambda\mathbf{I-B}\right)\overset{!}{=}0
	\quad&\rightarrow
	\begin{vmatrix}
	\lambda+\frac{1}{\sqrt{5}} & -\frac{2}{\sqrt{5}} \\
	-\frac{2}{\sqrt{5}} & \lambda-\frac{1}{\sqrt{5}}
	\end{vmatrix}
	\overset{!}{=}0& \\
	&\Rightarrow\lambda_{1}^{B}=1,\quad\lambda_{2}^{B}=-1&
\end{align*}

\subsection*{b) Determinant \& Trace}
\begin{align*}
	&\left|\mathbf{A}\right| =
	\begin{vmatrix}
	-1 & 1 \\
	1 & -1
	\end{vmatrix} = 1-1 = 0,\quad
	\left|\mathbf{B}\right| = -1& \\
	&\det\left(\mathbf{A}\right)=
	\begin{vmatrix}
	a_{11} & a_{12} & a_{13} \\
	a_{21} & a_{22} & a_{23} \\
	a_{31} & a_{32} & a_{33}
	\end{vmatrix}= a_{11}\left(-1\right)^{2}\left(a_{22}a_{33}-a_{32}a_{23}\right)+a_{12}\left(-1\right)^{2}\left(a_{21}a_{33}-a_{31}a_{23}\right)+\ldots& \\
	&\left|\mathbf{AB}\right|=\left|\mathbf{A}\right|\cdot\left|\mathbf{B}\right|\rightarrow\mathbf{AB}=\frac{1}{\sqrt{5}}
	\begin{pmatrix}
	3 & -1 \\
	-3 & 1
	\end{pmatrix}
	\rightarrow\left|\mathbf{AB}\right|=\frac{1}{5}\left(3-3\right)=0& \\
	&\tr\left(\mathbf{A}\right)=-1-1=-2,\quad\tr\left(\mathbf{B}\right)=0& \\
	&\lambda_{1}^{A}=-2,\quad\lambda_{2}^{A}=0\quad\rightarrow\quad\tr\left(\mathbf{A}\right)=\sum_{i}\lambda_{i}^{A}& \\
	&\lambda_{1}^{B}=1,\quad\lambda_{2}^{B}=-1\quad\rightarrow\quad\tr\left(\mathbf{B}\right)=\sum_{i}\lambda_{i}^{B}& \\
	&\left|\mathbf{A}\right|=\lambda_{1}^{A}\lambda_{2}^{A}=\prod_{i}\lambda_{i}^{A}&
\end{align*}

\subsection*{c)}
\begin{align*}
	&\tr\left(\mathbf{AB}\right)=\tr\left(\mathbf{BA}\right)\quad\forall\mathbf{A, B} \text{: square matrix N$\times$N}& \\
	&\mathbf{C=AB}\quad\rightarrow\quad c_{m,n}=\sum_{k}a_{m,k}b_{k,n}\quad\rightarrow\quad\tr\left(\mathbf{C}\right)=\sum_{i=1}^{N}c_{i,i}=\sum_{i=1}^{N}\sum_{k=1}^{N}a_{i,k}b_{k,i}& \\
	&\mathbf{D=BA}\quad\rightarrow\quad d_{m,n}=\sum_{k}b_{m,k}a_{k,n}\quad\rightarrow\quad\tr\left(\mathbf{D}\right)=\sum_{i=1}^{N}d_{i,i}=\sum_{i=1}^{N}\sum_{k=1}^{N}b_{i,k}a_{k,i}&
\end{align*}

\subsection*{d)}
\qquad\circled{1}
\begin{align*}
	&\text{positive definite matrix :}& &\text{$\forall i$, $\lambda_{i}>0$}& \\
	&\text{positive semidefinite matrix :}& &\text{$\forall i$, $\lambda_{i}\ge 0$}& \\
	&\text{negative definite matrix :}& &\text{$\forall i$, $\lambda_{i}<0$}& \\
	&\text{negative semidefinite matrix :}& &\text{$\forall i$, $\lambda_{i}\le 0$}& \\
	&\mathbf{A}:\quad\lambda_{i}^{A}\le 0\quad\Rightarrow\quad\text{negative semidefinite}& \\
	&\mathbf{B}:\quad\text{indefinite}&
\end{align*}
\qquad\circled{2}
\begin{align*}
	\mathbf{X}^{H}=\mathbf{X}\quad\rightarrow\quad\mathbf{X}^{T}=\mathbf{X}\quad\rightarrow\quad\mathbf{A, B}\text{: hermitian}
\end{align*}
\qquad\circled{3}
\begin{align*}
	&\rank\left(
	\begin{pmatrix}
	-1 & 1 \\
	1 & -1
	\end{pmatrix}
	\right)\rightarrow\rank\left(\mathbf{A}\right)=1& \\
	&\rank\left(\frac{1}{\sqrt{5}}
	\begin{pmatrix}
	-1 & 2 \\
	2 & 1
	\end{pmatrix}
	\right)=
	\rank\left(\frac{1}{\sqrt{5}}\left(\mathbf{b}_{1}\quad\mathbf{b}_{2}\right)\right)& \\
	&\beta_{1}\mathbf{b}_{1}+\beta_{2}\mathbf{b}_{2}=0\quad\rightarrow\quad
	\begin{pmatrix}-1\\2\end{pmatrix}+\beta_{2}\begin{pmatrix}2\\1\end{pmatrix}=\begin{pmatrix}0\\0\end{pmatrix}& \\
	&\Rightarrow\beta_{2}=-\frac{1}{2},\quad\beta_{2}=-2\quad\lightning& \\
	&\Rightarrow\quad\rank\left(\mathbf{B}\right)=2&
\end{align*}
\qquad\underline{Important property:}
\begin{align*}
	\mathbf{X}\text{ has full rank}\quad\rightarrow\quad\left|\mathbf{X}\right|\neq 0\text{ or $\mathbf{X}$ is invertible} \\
\end{align*}
\qquad\circled{4}
\begin{align*}
	&\left|\mathbf{A}\right|=0\quad\Rightarrow\quad\text{$\mathbf{A}$ nicht invertierbar}& \\
	&\left|\mathbf{B}\right|=-1\quad\Rightarrow\quad\text{$\mathbf{B}$ invertierbar}&
\end{align*}
\qquad\circled{5}
\begin{align*}
	&\mathbf{X}\text{ is unitary}\quad\Leftrightarrow\quad\mathbf{X\cdot X}^{H}=\mathbf{T},\quad\mathbf{X}\text{: unitary}\rightarrow\mathbf{X}^{-1}=\mathbf{X}^{H}& \\
	&\mathbf{AA}^{H}=
	\begin{pmatrix}
	-1 & 1 \\
	1 & -1
	\end{pmatrix}
	\begin{pmatrix}
	-1 & 1 \\
	1 & -1
	\end{pmatrix}=
	\begin{pmatrix}
	2 & -2 \\
	-2 & 2
	\end{pmatrix}&&\Rightarrow\mathbf{A}\text{ is not unitary}& \\
	&\mathbf{BB}^{H}=\frac{1}{5}
	\begin{pmatrix}
	-1 & 2 \\
	2 & 1
	\end{pmatrix}
	\begin{pmatrix}
	-1 & 2 \\
	2 & 1
	\end{pmatrix}=
	\begin{pmatrix}
	1 & 0 \\
	0 & 1
	\end{pmatrix}=\mathbf{I}&&\Rightarrow\mathbf{B}\text{ is unitary}&
\end{align*}

\subsection*{e) }
\begin{align*}
	&\left|\mathbf{I+AB}\right|=\left|\mathbf{I+BA}\right|& \\
	&\left|\mathbf{I+AB}\right|=\left|
	\begin{pmatrix}
	1 & 0 \\
	0 & 1
	\end{pmatrix}+\frac{1}{\sqrt{5}}
	\begin{pmatrix}
	3 & -1 \\
	-3 & 1
	\end{pmatrix}\right|=2,7789& \\
	&\left|\mathbf{I+BA}\right|=\left|
	\begin{pmatrix}
	1 & 0 \\
	0 & 1
	\end{pmatrix}+\frac{1}{\sqrt{5}}
	\begin{pmatrix}
	3 & -3 \\
	-1 & 1
	\end{pmatrix}\right|=2,7789& \\
	&&\blacksquare
\end{align*}

\subsection*{f) }
\begin{align*}
	&\mathbf{X}^{-1}=\frac{1}{\left|\mathbf{X}\right|}\adj\left(\mathbf{X}\right),\quad\adj\left(\mathbf{X}\right)=\text{ Transpose of cofactor matrix}& \\
	&\mathbf{X}=
	\begin{pmatrix}
	x_{11} & x_{12} & x_{13} \\
	x_{21} & x_{22} & x_{23} \\
	x_{31} & x_{32} & x_{33}
	\end{pmatrix}=\frac{1}{\det\mathbf{X}}
	\begin{pmatrix}
		\left(x_{22}x_{33}-x_{32}x_{23}\right) & \cdots & \cdots \\
		\cdots & \cdots & \cdots \\
		\cdots & \cdots & \cdots
	\end{pmatrix}& \\
	&\mathbf{B}=
	\begin{pmatrix}
	b_{11} & b_{12} \\
	b_{21} & b_{22}
	\end{pmatrix}& \\
	&\rightarrow\quad\mathbf{B}^{-1}=\frac{1}{\det\mathbf{B}}
	\begin{pmatrix}
	b_{22} & -b_{21} \\
	-b_{21} & b_{11}
	\end{pmatrix}^{T}=\frac{1}{-1}
	\begin{pmatrix}
	\frac{1}{\sqrt{5}} & -\frac{2}{\sqrt{5}} \\
	-\frac{2}{\sqrt{5}} & -\frac{1}{\sqrt{5}}
	\end{pmatrix}^{T}& \\
	&\rightarrow\quad\mathbf{B}^{-1}=
	\begin{pmatrix}
	-\frac{1}{\sqrt{5}} & \frac{2}{\sqrt{5}} \\
	\frac{2}{\sqrt{5}} & \frac{1}{\sqrt{5}}
	\end{pmatrix},\quad\left|\mathbf{B}^{-1}\right|=-1\quad\Rightarrow\left|\mathbf{B}^{-1}\right|=\frac{1}{\left|\mathbf{B}\right|}& \\
	&&\blacksquare
\end{align*}

\subsection*{g) }
\begin{align*}
	&\rank\left(\mathbf{A}\right)=1,\quad\rank\left(\mathbf{B}\right)=2& \\
	&\mathbf{AB}=\frac{1}{\sqrt{5}}
	\begin{pmatrix}
	3 & -1 \\
	-3 & 1
	\end{pmatrix},\quad
	\begin{pmatrix}3\\-3\end{pmatrix}=-3\begin{pmatrix}-1\\1\end{pmatrix}\quad\rightarrow\quad\rank\left(\mathbf{AB}\right)=1& \\
	&\rank\left(\mathbf{AB}\right)\le\min\{\rank\left(\mathbf{A}\right), \rank\left(\mathbf{B}\right)\}&
\end{align*}

\subsection*{h) }
\begin{align*}
	&\|\bullet\|: \mathbb{C}^{M\times N}\quad\rightarrow\quad\mathbb{R}& \\\\
	&\text{Axioms for norm function:}&\\
	&1.)\quad\|\mathbf{X}\|\ge 0,\quad\|\mathbf{X}\|=0 \text{ if and only if }\mathbf{X}=0& \\
	&2.)\quad\|\alpha\mathbf{X}\|=\left|\alpha\right|\|\mathbf{X}\|& \\
	&3.)\quad\|\mathbf{X+Y}\|\le\|\mathbf{X}\|+\|\mathbf{Y}\|& \text{(triangular property)} \\
	&4.)\quad\|\mathbf{XY}\|\le\|\mathbf{X}\|\cdot\|\mathbf{Y}\|&
\end{align*}

\subsection*{i)}
\begin{align*}
	&\|\alpha\mathbf{X}\|_{F}=\sqrt{\sum_{i}\sum_{j}\left|\alpha\mathbf{X}\right|^{2}}=\left|\alpha\right|\sqrt{\sum_{i}\sum_{j}\left|\mathbf{X}\right|^{2}}=\left|\alpha\right|\|\mathbf{X}\|_{F}& &\text{Axiom 2}& \\
	&\|\mathbf{X+Y}\|_{F}^{2}\le\|\mathbf{X}\|_{F}^{2}+\|\mathbf{Y}\|_{F}^{2}& &\text{Axiom 3}& \\
	&\|\mathbf{X+Y}\|_{F}^{2}=\sum_{i}\sum_{j}\left|x_{ij}+y_{ij}\right|^{2}& &\text{Axiom 4}& \\
	&\qquad\le\sum_{i}\sum_{j}\left|x_{ij}\right|^{2}+\sum_{i}\sum_{j}\left|y_{ij}\right|^{2}=\|\mathbf{X}\|_{F}^{2}+\|\mathbf{Y}_{F}^{2}& \\
	&\qquad\|\mathbf{XY}\|_{F}^{2}\le\|\mathbf{X}\|_{F}^{2}\cdot\|\mathbf{Y}\|_{F}^{2}& \\
	&\qquad\rightarrow\|\mathbf{XY}\|_{F}^{2}=\sum_{i}\sum_{j}\mathbf{XY}\le\sum_{i}\sum_{j}\left|x_{ij}\right|^{2}\cdot\sum_{i}\sum_{j}\left|y_{ij}\right|^{2}=\|\mathbf{X}\|_{F}^{2}\cdot\|\mathbf{Y}\|_{F}^{2} & \\
	& &\blacksquare
\end{align*}

\subsection*{j)}
\begin{align*}
	&\mathbf{A\otimes B\neq B\otimes A}& \\
	&\mathbf{A}=
	\begin{pmatrix}
	-1 & 1 \\
	1 & -1 
	\end{pmatrix},\quad\mathbf{B}=\frac{1}{\sqrt{5}}
	\begin{pmatrix}
	-1 & 2 \\
	2 & 1
	\end{pmatrix}& \\
	&\mathbf{A\otimes B}=
	\begin{bmatrix}
	a_{ij} & \mathbf{B}
	\end{bmatrix}=\frac{1}{\sqrt{5}}
	\begin{pmatrix}
	1 & 2 & -1 & 2 \\
	-2 & 1 & 2 & 1 \\
	-1 & 2 & 1 & -2 \\
	2 & 1 & -2 & -1
	\end{pmatrix}& \\
	&\mathbf{B\otimes A}=
	\begin{bmatrix}
	b_{ij} & \mathbf{A}
	\end{bmatrix}=\frac{1}{\sqrt{5}}
	\begin{pmatrix}
	1 & -1 & -2 & 2 \\
	-1 & 1 & 2 & -1 \\
	-2 & 2 & -1 & 1 \\
	2 & -2 & 1 & -1
	\end{pmatrix}& \\
	&\Rightarrow\mathbf{A\otimes B\neq B\otimes A}& \\
	& &\blacksquare
\end{align*}

\subsection*{k)}
\begin{align*}
	&\text{Hadamard's Inequality: }\left|\mathbf{A}\right|\le\prod_{k=1}^{K}a_{kk}& \\
	&\mathbf{A}=
	\begin{pmatrix}
	1 & 2 & -1 \\
	2 & -2 & -1 \\
	3 & 1 & 0
	\end{pmatrix}=1-2\left(3\right)-1\left(2+6\right)=-13& \\
	&\prod_{k=1}^{3}a_{kk}=0\quad\rightarrow\quad\det\left(\mathbf{A}\right)=-13\le\prod_{k=1}^{3}a_{kk}& \\
	&\tilde{\mathbf{A}}=
	\begin{pmatrix}
	1 & 0 & 0 \\
	0 & -2 & 0 \\
	0 & 0 & 0
	\end{pmatrix}\quad\rightarrow\quad\left|\tilde{\mathbf{A}}\right|=1\left(-2\right)0=0& \\
	&\qquad\rightarrow\text{off-diagonal elements should set to zero}\leftrightarrow\left|\mathbf{A}\right|=\prod_{k=1}^{K}a_{kk}&
\end{align*}